Update

Loda/AstTest.lean
@@ -116,7 +116,7 @@ example : Eval.eval σ0 δ0 123 sumIter = some (Ast.Value.vInt 6) := by
 def mulCircuit : Circuit.Circuit := {
   name   := "mul",
   inputs := [("x₁", Ast.Ty.field 7), ("x₂", Ast.Ty.field 7)],
-  output := ("out", Ast.Ty.refin (Ast.Ty.field 7) (expr_eq v (Ast.Expr.fieldExpr (Ast.Expr.var "x₁") Ast.FieldOp.mul (Ast.Expr.var "x₂")))),
+  output := ("out", Ast.Ty.refin (Ast.Ty.field 7) (Ast.expr_eq Ast.v (Ast.Expr.fieldExpr (Ast.Expr.var "x₁") Ast.FieldOp.mul (Ast.Expr.var "x₂")))),
   body   := (Ast.Expr.fieldExpr (Ast.Expr.var "x₁") Ast.FieldOp.mul (Ast.Expr.var "x₂"))
 }
 
@@ -125,10 +125,10 @@ def env35 : Env.ValEnv := fun x =>
   if x = "x₁" then Ast.Value.vF 7 3 else if x = "x₂" then Ast.Value.vF 7 5 else Ast.Value.vStar
 def Γ0 : Env.TyEnv := fun _ => Ast.Ty.field 7
 
-#check circuit2prop 7 testEnv mulCircuit
+#check PropSemantics.circuit2prop 7 testEnv mulCircuit
 
-theorem mulCircuit_correct : (circuit2prop 7 testEnv mulCircuit) := by
-  unfold circuit2prop
+theorem mulCircuit_correct : (PropSemantics.circuit2prop 7 testEnv mulCircuit) := by
+  unfold PropSemantics.circuit2prop
   intros xs hlen
   cases xs
   case nil =>
